\begin{enumerate}
    \item \(\sum_{i=1}^{n} 1 = n\)
    \vspace{0.15cm}
    \item \(\sum_{i=1}^{n} i = \frac{n(n+1)}{2}\)
    \vspace{0.15cm}
    \item \(\sum_{i=1}^{n} i^2 = \frac{n(n+1)(2n+1)}{6}\)
    \vspace{0.15cm}
    \item \(\sum_{i=1}^{n} i^3 =  (\sum_{i=1}^{n} i)^2  \)
    \vspace{0.15cm}
    \item \(\sum_{i=0}^{k} 2^i =  2^{k+1} - 1  \)
    \vspace{0.15cm}
    \item \(\sum_{i=0}^{k} \frac{1}{2^i} =  2\)\hspace{0.15cm} when \(k \to +\infty\)
    \vspace{0.15cm}
    \item \(\sum_{i=0}^{n} x^i =  \frac{x^{n+1}-1}{x-1}\)\hspace{0.15cm} with \(x \neq 1\)
    \vspace{0.15cm}
    \item \(\sum_{k=1}^{n} \frac{1}{k} =  1+\frac{1}{2}+\frac{1}{3}+\dots+\frac{1}{n} \sim \ln(n) \)
    \vspace{0.15cm}
    \item \(\log(n!) \sim n\log(n)\)
    \vspace{0.15cm}
    \item \(\lim\limits_{n\to +\infty} \sum_{k = 0}^n x^k  = \frac{1}{1-x}\)\hspace{0.15cm} if \(|x| < 1\) 
    \vspace{0.15cm}                                                                    
    \item \(\sum_{i = 0}^n ix^i  = \frac{1}{(1-x)^2}\)\hspace{0.15cm} if \(|x| < 1\) 
    \vspace{0.15cm}
    \item \(\log(ab) = \log(a) + \log(b)\)
    \vspace{0.15cm}
    \item \(\log(\frac{a}{b}) = \log(a) - \log(b)\) 
    \vspace{0.15cm}
    \item \(\log(a^b) = b\log(a)\)
    \vspace{0.15cm}
    \item \(\log_b(a) = \frac{\ln(a)}{\ln(b)}\) 
    \vspace{0.15cm}
    \item \(a^{\log_b(n)} = n^{\log_b(a)}\) 
    \vspace{0.15cm}
    \item \(a^n\times a^m = a^{n+m}\)
    \vspace{0.15cm}
    \item \((a^m)^n = a^{m*n}\)
    \vspace{0.15cm}
\item \(a^{(m)^{n}} \neq (a^{m})^n\)
\end{enumerate}
